new infrastructure lemmas

FzipCore/FzipCore_init.v
@@ -29,7 +29,7 @@ Ltac size_absurd size t :=
 Ltac size_term_absurd t := size_absurd size_term t.
 
 (** env_map *)
-Definition tag_map {A B : Set} (f : A → B) (t : @tag A) :=
+Definition tag_map {A B : Type} (f : A → B) (t : @tag A) :=
   match t with
     | U => U
     | E => E
@@ -38,9 +38,67 @@ Definition tag_map {A B : Set} (f : A → B) (t : @tag A) :=
   end.
 Hint Unfold tag_map.
 
-Definition env_map {A : Set} (f : typ → A) (env : typing_env) :=
+Definition env_map {A : Type} (f : typ → A) (env : typing_env) :=
   map (tag_map f) env.
 Hint Unfold env_map.
+
+Definition binding_fold {A B : Type} (f : B → A → B)  (acc : B) (b : atom * @tag A) :=
+  match b with
+    | (_, U) => acc
+    | (_, E) => acc
+    | (_, T a) => f acc a
+    | (_, Eq a) => f acc a
+  end.
+Hint Unfold binding_fold.
+
+Definition env_fold {A : Type} (f : A → typ → A) (env : typing_env) (acc : A) :=
+  fold_left (binding_fold f) env acc.
+Hint Unfold env_fold.
+
+Definition ftv_env (G : typing_env) :=
+  env_fold (fun acc t => ftv_typ t ∪ acc) G {}.
+Hint Unfold ftv_env.
+
+Lemma ftv_env_nil : ftv_env nil [=] {}.
+Proof.
+reflexivity.
+Qed.
+
+Lemma ftv_env_app_aux (G : typing_env) (s : atoms) :
+  env_fold (fun acc t => ftv_typ t ∪ acc) G s [=] ftv_env G ∪ s.
+Proof.
+intros G. induction G; intros; simpl in *.
+fsetdec.
+destruct a; destruct t;
+unfold ftv_env; simpl; repeat rewrite IHG; fsetdec.
+Qed.
+
+Lemma ftv_env_app (G1 G2 : typing_env) :
+  ftv_env (G1 ++ G2) [=] ftv_env G1 ∪ ftv_env G2.
+Proof.
+intro G1. induction G1; intros; simpl_env in *.
+fsetdec.
+destruct a. unfold ftv_env. destruct t; simpl;
+repeat rewrite ftv_env_app_aux; rewrite IHG1; fsetdec.
+Qed.
+Hint Rewrite ftv_env_nil ftv_env_app : lngen.
+
+Lemma tsubst_env_fresh_eq :
+forall G t a,
+  a ∉ ftv_env G ->
+  env_map (tsubst_typ t a) G = G.
+Proof.
+intros G t a H.
+induction G; simpl in *; simpl_env in *.
+auto.
+autorewrite with lngen in *.
+f_equal; auto.
+destruct a0; destruct t0; auto.
+assert (a ∉ ftv_typ t0). unfold ftv_env in H; simpl in H; auto.
+simpl; autorewrite with lngen; auto.
+assert (a ∉ ftv_typ t0). unfold ftv_env in H; simpl in H; auto.
+simpl; autorewrite with lngen; auto.
+Qed.
 
 (** Additional lemmas *)
 Lemma var_subst : forall e x, subst_term e x (term_var_f x) = e.
@@ -54,3 +112,59 @@ Proof.
 intros t a; simpl; destruct (a == a); congruence.
 Qed.
 Hint Rewrite tvar_tsubst : lngen.
+
+Lemma tsubst_typ_var_twice :
+  forall τ a b,
+    lc_typ τ →
+    a ∉ ftv_typ τ →
+    tsubst_typ (typ_var_f b) a (tsubst_typ (typ_var_f a) b τ) = τ.
+Proof.
+intros τ a b H H0.
+induction H; simpl in *; try solve [f_equal; auto].
+Case "var". destruct (a0 == b); subst.
+SCase "a0 = b". rewrite tvar_tsubst. auto.
+SCase "a0 ≠ b". simpl. destruct (a0 == a); subst; auto.
+SSCase "a0 = a". simpl in H0. elimtype False; auto.
+Case "forall". f_equal. pick fresh c.
+  apply open_typ_wrt_typ_inj with (a1 := c); auto.
+  assert (ftv_typ (tsubst_typ (typ_var_f b) a (tsubst_typ (typ_var_f a) b t))
+    [<=] ftv_typ (typ_var_f b) ∪ remove a (ftv_typ (tsubst_typ (typ_var_f a) b t)))
+  by auto with lngen.
+  assert (ftv_typ (tsubst_typ (typ_var_f a) b t) [<=] ftv_typ (typ_var_f a) ∪ remove b (ftv_typ t))
+    by auto with lngen.
+  simpl in *; fsetdec.
+  repeat rewrite tsubst_typ_open_typ_wrt_typ_var; auto. apply H1.
+  assert (ftv_typ (open_typ_wrt_typ t (typ_var_f c)) [<=]
+    ftv_typ (typ_var_f c) ∪ ftv_typ t) by auto with lngen.
+  simpl in *. fsetdec.
+Case "exists". f_equal. pick fresh c.
+  apply open_typ_wrt_typ_inj with (a1 := c); auto.
+  assert (ftv_typ (tsubst_typ (typ_var_f b) a (tsubst_typ (typ_var_f a) b t))
+    [<=] ftv_typ (typ_var_f b) ∪ remove a (ftv_typ (tsubst_typ (typ_var_f a) b t)))
+  by auto with lngen.
+  assert (ftv_typ (tsubst_typ (typ_var_f a) b t) [<=] ftv_typ (typ_var_f a) ∪ remove b (ftv_typ t))
+    by auto with lngen.
+  simpl in *; fsetdec.
+  repeat rewrite tsubst_typ_open_typ_wrt_typ_var; auto. apply H1.
+  assert (ftv_typ (open_typ_wrt_typ t (typ_var_f c)) [<=]
+    ftv_typ (typ_var_f c) ∪ ftv_typ t) by auto with lngen.
+  simpl in *. fsetdec.
+Qed.
+
+Lemma tsubst_typ_lc_typ_inv :
+  forall t1 a1 t2,
+    lc_typ t1 →
+    lc_typ (tsubst_typ t1 a1 t2) →
+    lc_typ t2.
+Proof.
+intros t1 a1.
+assert (forall n m t2, size_typ t2 <= n →
+  degree_typ_wrt_typ m (tsubst_typ t1 a1 t2) →
+  degree_typ_wrt_typ m t2) as H_strong.
+  intro n; induction n; intros m t2 H H0;
+    destruct t2; simpl in *;
+      try solve [absurdity with omega |
+      inversion H0; subst; constructor; apply IHn; try omega; auto].
+  auto.
+intros t2 H H0. eauto with lngen.
+Qed.
